feat: add several definitions and theorems about reduction systems (#211)
This PR adds some additional API to `ReductionSystem`. While it
duplicates from the relation namespace, this seems like an acceptable
tradeoff for unifying proofs that use the corresponding notation, and
ultimately a user can still simplify to the underlying relation if they
desire. (description added by Chris Henson)

---------

Co-authored-by: Chris Henson <chrishenson.net@gmail.com>

Cslib/Foundations/Semantics/ReductionSystem/Basic.lean
@@ -7,7 +7,7 @@ Authors: Fabrizio Montesi, Thomas Waring
 module
 
 public import Cslib.Init
-public import Mathlib.Logic.Relation
+public import Cslib.Foundations.Data.Relation
 public import Mathlib.Util.Notation3
 
 @[expose] public section
@@ -30,25 +30,173 @@ structure ReductionSystem (Term : Type u) where
   Red : Term → Term → Prop
 
 
+variable {Term : Type u} (rs : ReductionSystem Term)
+
 section MultiStep
 
 /-! ## Multi-step reductions -/
 
 /-- Multi-step reduction relation. -/
-abbrev ReductionSystem.MRed (rs : ReductionSystem Term) :=
+abbrev ReductionSystem.MRed :=
   Relation.ReflTransGen rs.Red
 
 /-- All multi-step reduction relations are reflexive. -/
 @[refl]
-theorem ReductionSystem.MRed.refl (rs : ReductionSystem Term) (t : Term) : rs.MRed t t :=
+theorem ReductionSystem.MRed.refl (t : Term) : rs.MRed t t :=
   Relation.ReflTransGen.refl
 
 /-- Any reduction is a multi-step -/
-theorem ReductionSystem.MRed.single (rs : ReductionSystem Term) (h : rs.Red a b) :
-  rs.MRed a b :=
+theorem ReductionSystem.MRed.single {a b : Term} (h : rs.Red a b) : rs.MRed a b :=
   Relation.ReflTransGen.single h
 
+theorem ReductionSystem.MRed.step {a b c : Term} (hab : rs.MRed a b) (hbc : rs.Red b c) :
+    rs.MRed a c :=
+  Relation.ReflTransGen.tail hab hbc
+
+theorem ReductionSystem.MRed.trans {a b c : Term} (hab : rs.MRed a b) (hbc : rs.MRed b c) :
+    rs.MRed a c :=
+  Relation.ReflTransGen.trans hab hbc
+
+theorem ReductionSystem.MRed.cases_iff {a b : Term} :
+    rs.MRed a b ↔ b = a ∨ ∃ c : Term, rs.MRed a c ∧ rs.Red c b :=
+  Relation.ReflTransGen.cases_tail_iff rs.Red a b
+
+@[induction_eliminator]
+theorem ReductionSystem.MRed.induction_on {motive : ∀ {x y}, rs.MRed x y → Prop}
+    (refl : ∀ t : Term, motive (MRed.refl rs t))
+    (step : ∀ (a b c : Term) (hab : rs.MRed a b) (hbc : rs.Red b c), motive hab →
+      motive (MRed.step rs hab hbc))
+    {a b : Term} (h : rs.MRed a b) : motive h := by
+  apply Relation.ReflTransGen.rec <;> grind
+
 end MultiStep
+
+
+section Reverse
+
+/-- Reverse reduction relation -/
+def ReductionSystem.RRed : Term → Term → Prop :=
+  Function.swap rs.Red
+
+theorem ReductionSystem.RRed.single {a b : Term} (h : rs.Red a b) : rs.RRed b a := h
+
+end Reverse
+
+section Equivalence
+
+/-- Equivalence closure relation -/
+def ReductionSystem.Eqv : Term → Term → Prop := Relation.EqvGen rs.Red
+
+theorem ReductionSystem.Eqv.refl (t : Term) : rs.Eqv t t :=
+  Relation.EqvGen.refl t
+
+theorem ReductionSystem.Eqv.single {a b : Term} (h : rs.Red a b) : rs.Eqv a b :=
+  Relation.EqvGen.rel a b h
+
+theorem ReductionSystem.Eqv.symm {a b : Term} (h : rs.Eqv a b) : rs.Eqv b a :=
+  Relation.EqvGen.symm a b h
+
+theorem ReductionSystem.Eqv.trans {a b c : Term} (h₁ : rs.Eqv a b) (h₂ : rs.Eqv b c) :
+    rs.Eqv a c :=
+  Relation.EqvGen.trans a b c h₁ h₂
+
+theorem ReductionSystem.Eqv.ofMRed {a b : Term} (h : rs.MRed a b) : rs.Eqv a b :=
+  Relation.ReflTransGen.to_eqvGen h
+
+@[induction_eliminator]
+theorem ReductionSystem.Eqv.induction_on {motive : ∀ {x y}, rs.Eqv x y → Prop}
+    (rel : ∀ (a b : Term) (hab : rs.Red a b), motive (Eqv.single rs hab))
+    (refl : ∀ t : Term, motive (Eqv.refl rs t))
+    (symm : ∀ (a b : Term) (hab : rs.Eqv a b), motive hab → motive (Eqv.symm rs hab))
+    (trans : ∀ (a b c : Term) (hab : rs.Eqv a b) (hbc : rs.Eqv b c), motive hab → motive hbc →
+      motive (Eqv.trans rs hab hbc))
+    {a b : Term} (h : rs.Eqv a b) : motive h := by
+  apply Relation.EqvGen.rec <;> grind
+
+end Equivalence
+
+section Join
+
+/-- Join relation -/
+def ReductionSystem.Join : Term → Term → Prop :=
+  Relation.Join rs.Red
+
+theorem ReductionSystem.Join_def {a b : Term} :
+    rs.Join a b ↔ ∃ c : Term, rs.Red a c ∧ rs.Red b c := by rfl
+
+theorem ReductionSystem.Join.symm : Symmetric rs.Join := Relation.symmetric_join
+
+end Join
+
+section MJoin
+
+/-- Multi-step join relation -/
+def ReductionSystem.MJoin : Term → Term → Prop :=
+  Relation.Join rs.MRed
+
+theorem ReductionSystem.MJoin_def {a b : Term} :
+    rs.MJoin a b ↔ ∃ c : Term, rs.MRed a c ∧ rs.MRed b c := by rfl
+
+theorem ReductionSystem.MJoin.refl (t : Term) : rs.MJoin t t := by
+  use t
+
+theorem ReductionSystem.MJoin.symm : Symmetric rs.MJoin := Relation.symmetric_join
+
+end MJoin
+
+/-- A reduction system has the diamond property when all one-step reduction pairs with a common
+origin are joinable -/
+def ReductionSystem.Diamond : Prop :=
+  Relation.Diamond rs.Red
+
+theorem ReductionSystem.isDiamond_def : rs.Diamond ↔
+    ∀ {a b c : Term}, rs.Red a b → rs.Red a c → rs.Join b c :=
+  Iff.rfl
+
+/-- A reduction system is confluent when all multi-step reduction pairs with a common origin are
+multi-step joinable -/
+def ReductionSystem.Confluent : Prop :=
+  Relation.Confluent rs.Red
+
+theorem ReductionSystem.Confluent_def : rs.Confluent ↔
+    ∀ {a b c : Term}, rs.MRed a b → rs.MRed a c → rs.MJoin b c :=
+  Iff.rfl
+
+/-- A reduction system is Church-Rosser when all equivalent terms are multi-step joinable -/
+def ReductionSystem.ChurchRosser : Prop := Relation.ChurchRosser rs.Red
+
+/-- A term is reducible when there exists a one-step reduction from it. -/
+def ReductionSystem.Reducible (t : Term) : Prop := Relation.Reducible rs.Red t
+
+/-- A term is in normal form when it is not reducible. -/
+def ReductionSystem.Normal (t : Term) : Prop := ¬ rs.Reducible t
+
+/-- A reduction system is normalizing when every term reduces to at least one normal form. -/
+def ReductionSystem.Normalizing : Prop :=
+  ∀ t : Term, ∃ n : Term, rs.MRed t n ∧ rs.Normal n
+
+/-- A reduction system is terminating when there are no infinite sequences of one-step reductions.
+-/
+def ReductionSystem.Terminating : Prop := Relation.Terminating rs.Red
+
+theorem ReductionSystem.isConfluent_iff_isChurchRosser : rs.Confluent ↔ rs.ChurchRosser :=
+  Relation.Confluent_iff_ChurchRosser
+
+theorem ReductionSystem.isTerminating_iff_WellFounded : rs.Terminating ↔ WellFounded rs.RRed := by
+  rfl
+
+theorem ReductionSystem.isNormalizing_of_isTerminating (h : rs.Terminating) :
+    rs.Normalizing := by
+  rw [isTerminating_iff_WellFounded] at h
+  intro t
+  apply WellFounded.induction h t
+  intro a ih
+  by_cases ha : rs.Reducible a
+  · obtain ⟨b, hab⟩ := ha
+    obtain ⟨n, hbn, hn⟩ := ih b hab
+    exact ⟨n, MRed.trans rs (MRed.single rs hab) hbn, hn⟩
+  · unfold Normal
+    use a
 
 open Lean Elab Meta Command Term
 
@@ -116,7 +264,7 @@ macro_rules
   This attribute calls the `reduction_notation` command for the annotated declaration, such as in:
 
   ```
-  @[reduction rs "ₙ", simp]
+  @[reduction_sys rs "ₙ", simp]
   def PredReduction (a b : ℕ) : Prop := a = b + 1
   ```
 -/
