Cslib/Languages/LambdaCalculus/LocallyNameless/Untyped/FullBeta.lean
@@ -65,14 +65,14 @@ lemma step_lc_l (step : M ⭢βᶠ M') : LC M := by
 theorem redex_app_l_cong (redex : M ↠βᶠ M') (lc_N : LC N) : app M N ↠βᶠ app M' N := by
   induction redex
   case refl => rfl
-  case tail ih r => exact Relation.ReflTransGen.tail r (appR lc_N ih)
+  case step a b c hab hbc ih => exact ReductionSystem.MRed.step fullBetaRs ih (appR lc_N hbc)
 
 /-- Right congruence rule for application in multiple reduction. -/
 @[scoped grind ←]
 theorem redex_app_r_cong (redex : M ↠βᶠ M') (lc_N : LC N) : app N M ↠βᶠ app N M' := by
   induction redex
   case refl => rfl
-  case tail ih r => exact Relation.ReflTransGen.tail r (appL lc_N ih)
+  case step ih r => exact Relation.ReflTransGen.tail r (appL lc_N ih)
 
 variable [HasFresh Var] [DecidableEq Var]
 
@@ -104,7 +104,7 @@ lemma redex_abs_close {x : Var} (step : M ↠βᶠ M') : (M⟦0 ↜ x⟧.abs ↠
   induction step using Relation.ReflTransGen.trans_induction_on
   case refl => rfl
   case single ih => exact Relation.ReflTransGen.single (step_abs_close ih)
-  case trans l r => exact .trans l r
+  case trans l r => exact Relation.ReflTransGen.trans l r
 
 /-- Multiple reduction of opening implies multiple reduction of abstraction. -/
 theorem redex_abs_cong (xs : Finset Var) (cofin : ∀ x ∉ xs, (M ^ fvar x) ↠βᶠ (M' ^ fvar x)) :
